theories/opt/ex1.v
@@ -3,27 +3,27 @@ From stbor.sim Require Import local invariant refl_step.
 Set Default Proof Using "Type".
 
 (* Assuming x : &mut i32 *)
-Definition ex1 : expr :=
-  let: "x" := new_place (&mut int) &"i" in
-  Retag "x" Default ;;
-  Call #[ScFnPtr "f"] [] ;;
-  *{int} "x" <- #[42] ;;
-  Call #[ScFnPtr "g"] [] ;;
-  Copy *{int} "x"
+Definition ex1 : function :=
+  fun: ["i"],
+    let: "x" := new_place (&mut int) &"i" in
+    Retag "x" Default ;;
+    Call #[ScFnPtr "f"] [] ;;
+    *{int} "x" <- #[42] ;;
+    Call #[ScFnPtr "g"] [] ;;
+    Copy *{int} "x"
   .
 
-Definition ex1_opt : expr :=
-  let: "x" := new_place (&mut int) &"i" in
-  Retag "x" Default ;;
-  Call #[ScFnPtr "f"] [] ;;
-  *{int} "x" <- #[42] ;;
-  let: "v" := Copy *{int} "x" in
-  Call #[ScFnPtr "g"] [] ;;
-  "v"
+Definition ex1_opt : function :=
+  fun: ["i"],
+    let: "x" := new_place (&mut int) &"i" in
+    Retag "x" Default ;;
+    Call #[ScFnPtr "f"] [] ;;
+    *{int} "x" <- #[42] ;;
+    let: "v" := Copy *{int} "x" in
+    Call #[ScFnPtr "g"] [] ;;
+    "v"
   .
 
-Lemma ex1_sim_body fs ft r n σs σt :
-  (* TODO: what's in r? *)
-  r ⊨{n, fs,ft} (ex1, σs) ≥ (ex1_opt, σt) : (λ r' _ vs' σs' vt' σt', vrel_expr r' vs' vt').
+Lemma ex1_sim_body fs ft : ⊨{fs,ft} ex1 ≥ᶠ ex1_opt.
 Proof.
 Abort.
