theories/opt/ex2.v
@@ -3,25 +3,25 @@ From stbor.sim Require Import local invariant refl_step.
 Set Default Proof Using "Type".
 
 (* Assuming x : & i32 *)
-Definition ex2 : expr :=
-  let: "x" := new_place (& int) &"i" in
-  Retag "x" Default ;;
-  Copy *{int} "x" ;;
-  Call #[ScFnPtr "f"] ["x"] ;;
-  Copy *{int} "x"
+Definition ex2 : function :=
+  fun: ["i"],
+    let: "x" := new_place (& int) &"i" in
+    Retag "x" Default ;;
+    Copy *{int} "x" ;;
+    Call #[ScFnPtr "f"] ["x"] ;;
+    Copy *{int} "x"
   .
 
-Definition ex2_opt : expr :=
-  let: "x" := new_place (& int) &"i" in
-  Retag "x" Default ;;
-  Copy *{int} "x" ;;
-  let: "v" := Copy *{int} "x" in
-  Call #[ScFnPtr "f"] ["x"] ;;
-  "v"
+Definition ex2_opt : function :=
+  fun: ["i"],
+    let: "x" := new_place (& int) &"i" in
+    Retag "x" Default ;;
+    Copy *{int} "x" ;;
+    let: "v" := Copy *{int} "x" in
+    Call #[ScFnPtr "f"] ["x"] ;;
+    "v"
   .
 
-Lemma ex2_sim_body fs ft r n σs σt :
-  (* TODO: what's in r? *)
-  r ⊨{n, fs,ft} (ex2, σs) ≥ (ex2_opt, σt) : (λ r' _ vs' σs' vt' σt', vrel_expr r' vs' vt').
+Lemma ex2_sim_body fs ft : ⊨{fs,ft} ex2 ≥ᶠ ex2_opt.
 Proof.
 Abort.
