theories/sim/left_step.v
@@ -1,0 +1,33 @@
+From iris.algebra Require Import local_updates.
+
+From stbor.lang Require Import steps_progress steps_inversion steps_retag.
+From stbor.sim Require Export instance.
+
+Set Default Proof Using "Type".
+
+Lemma sim_body_copy_left_1
+  fs ft (r: resUR) k (h: heapletR) n l t et σs σt Φ
+  (UNIQUE: r.1 !! t ≡ Some (k, h))
+  (InD: l ∈ dom (gset loc) h) :
+  (∀ s, σs.(shp) !! l = Some s → r ⊨{n,fs,ft} (#[s%S], σs) ≥ (et, σt) : Φ : Prop) →
+  r ⊨{n,fs,ft} (Copy (Place l (Tagged t) int), σs) ≥ (et, σt) : Φ.
+Proof.
+  intros COND. pfold. intros NT r_f WSAT.
+  edestruct NT as [[]|[es1 [σs1 STEP1]]]; [constructor 1|done|].
+  destruct (tstep_copy_inv _ _ _ _ _ _ _ STEP1) as (vs & α' & ? & Eqvs & READ & ?).
+  subst es1 σs1. rewrite /= read_mem_equation_1 /= in Eqvs.
+  destruct (σs.(shp) !! l) as [s|] eqn:Eqs; [|done]. simpl in Eqvs. simplify_eq.
+  specialize (COND _ eq_refl).
+
+  (* we need to invoke WSAT to know that α' = σs.(sst) *)
+  destruct WSAT as (WFS & WFT & VALID & PINV & CINV & SREL).
+
+  (* once we know that the state did not change, we can use COND. *)
+  have NT2 := never_stuck_tstep_once _ _ _ _ _ STEP1 NT.
+  punfold COND.
+
+  split.
+  { (* this comes from COND *) admit. }
+  { (* follows COND *) admit. }
+  { (* follows COND *) admit. }
+Abort.
