theories/sim/right_step.v
@@ -1,0 +1,17 @@
+From iris.algebra Require Import local_updates.
+
+From stbor.lang Require Import steps_progress steps_inversion steps_retag.
+From stbor.sim Require Export instance.
+
+Set Default Proof Using "Type".
+
+Lemma sim_body_copy_right_1
+  fs ft (r: resUR) k (h: heapletR) n l t s es σs σt Φ
+  (* we know we're going to read s *)
+  (UNIQUE: r.1 !! t ≡ Some (k, h))
+  (InD: h !! l ≡ Some (to_agree s))
+  (IN: tag_in_stack σt l t) :
+  (σt.(shp) !! l = Some s → r ⊨{n,fs,ft} (es, σs) ≥ (#[s%S], σt) : Φ : Prop) →
+  r ⊨{n,fs,ft} (es, σs) ≥ (Copy (Place l (Tagged t) int), σt) : Φ.
+Proof.
+Abort.
